Experiment with locally nameless

lean/src/puddle/syntax.lean
@@ -1,40 +1,140 @@
+import .except
+import struct_tact
+
+namespace puddle
+namespace syntax
+
+@[derive(decidable_eq)]
 inductive type : Type
 | unit
 
-def context := list (string × type)
+def type.mix (t1 t2 : type) : except string type :=
+except.error "foo"
 
-/- The polymoprhic term type representing our syntax, we use
-   PHOAS to implement the name binding.
--/
-inductive pterm (v : Type) /- :context → type → -/ : Type
-| var : v → pterm
-| input : pterm
-| output : pterm → pterm
-| mix : pterm → pterm → pterm
-| bind : pterm → (v → pterm) → pterm
+/- The term type representing our terms implemented
+   using a locally nameless representation. -/
+inductive term : Type
+| free : string → type → term
+| var : nat → term
+| input : type → term
+| output : term → term
+| mix : term → term → term
+| bind : string → type → term → term → term
 
--- output (if cond then d1 else d2)
+namespace term
 
--- if cond:
---   x = d1
--- else:
---   x = d2
---
--- output x
+/-- A term is closed, i.e there are no dangling `var`s. -/
+inductive is_closed' : term → nat → Prop
+| free : forall s t n,
+    is_closed' (term.free s t) n
+| var : forall n m,
+    n < m →
+    is_closed' (term.var n) m
+| input : forall ty n, is_closed' (term.input ty) n
+| output : forall t m,
+    is_closed' t m →
+    is_closed' (term.output t) m
+| mix : forall n t1 t2,
+    is_closed' t1 n →
+    is_closed' t2 n →
+    is_closed' (mix t1 t2) n
+| bind : forall x v ty body n,
+    is_closed' v n →
+    is_closed' body (n + 1) →
+    is_closed' (term.bind x ty v body) n
 
-def term := pterm string
+def is_closed (t : term) : Prop :=
+is_closed' t 0
 
-open pterm
+def abstract_aux (name : string) : nat → term → term
+| outer (term.free name' ty) :=
+    if name = name'
+    then term.var outer
+    else term.free name' ty
+| outer (term.var b) := term.var b
+| outer (term.input ty) := (term.input ty)
+| outer (term.output d) :=
+  term.output (abstract_aux outer d)
+| outer (term.mix d1 d2) :=
+  term.mix (abstract_aux outer d1) (abstract_aux outer d2)
+| outer (term.bind x ty v body) :=
+  term.bind x ty (abstract_aux outer v) (abstract_aux (outer + 1) body)
 
-def mix_out : term :=
-    (pterm.bind (pterm.input _) $
-        (fun d1, pterm.bind (pterm.input _)  $
-            (fun d2, output (mix (var d1) (var d2)))))
+def abstract (n : string) (t : term) : term :=
+abstract_aux n 0 t
 
-/-
-    d1 = input()
-    d2 = input()
-    d3 = mix d1 d2
-    r = output(d3)
-    return r
--/
+def instantiate_aux (image : term) : nat → term → term
+| outer (term.var index) :=
+    if index = outer
+    then image
+    else term.var index
+| outer (term.free name ty) := term.free name ty
+| outer (term.output d) := term.output (instantiate_aux outer d)
+| outer (term.mix d1 d2) :=
+  term.mix (instantiate_aux outer d1) (instantiate_aux outer d2)
+| outer (term.input ty) := term.input ty
+| outer (term.bind x ty v body) :=
+  term.bind x ty
+    (instantiate_aux outer v)
+    (instantiate_aux (outer + 1) body)
+
+def instantiate (sub : term) (target : term) : term :=
+instantiate_aux sub 0 target
+
+lemma instantiate_abstract_aux :
+∀ (name : string) (t : term) (ty : type) i,
+    is_closed t →
+    instantiate_aux (free name ty) i (abstract_aux name i t) = t :=
+begin
+    intros name t, induction t; intros,
+    { simp [abstract_aux, instantiate_aux],
+      by_cases (name = t_a); simp * at *,
+      { simp [abstract_aux, instantiate_aux],
+        constructor, trivial,
+      },
+      { existsi type.unit, simp [instantiate_aux] }
+    },
+    { simp [is_closed] at a,
+      cases t, cases a, cases a_a,
+      cases a, cases a_a,
+    },
+    { simp [abstract_aux, instantiate_aux], existsi type.unit,
+      trivial,
+    },
+    { cases a,
+      cases (t_ih a_a),
+      existsi _,
+      simp [abstract_aux, instantiate_aux],
+      rw h,
+    },
+    { cases a,
+      cases (t_ih_a a_a),
+      cases (t_ih_a_1 a_a_1),
+      simp [abstract_aux, instantiate_aux],
+      constructor,
+      simp * at *,
+      admit,
+      admit,
+    },
+    { admit }
+end
+
+lemma instantiate_abstract :
+forall name t,
+  exists ty,
+    term.instantiate (term.free name ty) (term.abstract name t) = t :=
+begin
+    intros, induction t,
+    { admit },
+    { simp [abstract, instantiate], },
+    { admit },
+end
+
+-- lemma instantiate_abstract :
+-- forall name t,
+--     instantiate
+
+end term
+
+end syntax
+end puddle
