lean/src/puddle/checker.lean
@@ -1,0 +1,56 @@
+import struct_tact
+import .syntax
+import .except
+
+namespace puddle
+namespace checker
+
+open puddle.syntax
+
+def context := list (string × type)
+def context.empty : context := []
+
+def context.lookup : context → string → option type
+| cx k := none
+
+def context.extend : context → context → context
+| cx cx' := cx
+
+-- #check well_founded_tactics.dec_tac
+
+def err := string
+
+mutual def check, infer
+with check : term → type → except err type
+| t expected :=
+    do t ← infer t,
+       if t = expected
+       then except.ok t
+       else except.error "mismatch"
+with infer : term → except err type
+| (term.free x ty) := except.ok ty
+| (term.var x) := except.error "can't type var"
+| (term.bind x ty v body) :=
+   do ty' ← check v ty, -- we might need the normalized type here
+      infer (term.instantiate (term.free x ty') body)
+| (term.input t) := except.ok t
+| (term.mix d1 d2) :=
+do t1 ← infer d1,
+   t2 ← infer d2,
+   type.mix t1 t2
+| (term.output d) := except.ok type.unit
+using_well_founded { dec_tac := tactic.admit }
+
+inductive typed : term → type → Prop
+| output : forall d, typed (term.output d) type.unit
+| input : forall ty, typed (term.input ty) ty
+| mix : forall d1 d2 ty1 ty2 ty3,
+    typed d1 ty1 →
+    typed d2 ty2 →
+    (type.mix ty1 ty2) = except.ok ty3 →
+    typed (term.mix d1 d2) ty3
+| free : forall x ty,
+    typed (term.free x ty) ty
+
+end checker
+end puddle
