lean/src/puddle/puddle_def.lean
@@ -1,0 +1,35 @@
+
+import .syntax
+
+#check tactic.coinduction
+
+namespace puddle
+namespace puddle_def
+
+open lean.parser
+open interactive
+open syntax
+
+meta def puddle_body : lean.parser term := sorry
+
+--   decl ← inductive_decl.parse meta_info,
+--   add_coinductive_predicate decl.u_names decl.params $ decl.decls.map $ λ d, (d.sig, d.intros),
+--   decl.decls.mmap' $ λ d, do {
+--     get_env >>= λ env, set_env $ env.add_namespace d.name,
+--     meta_info.attrs.apply d.name,
+--     d.attrs.apply d.name,
+--     some doc_string ← pure meta_info.doc_string | skip,
+--     add_doc_string d.name doc_string
+--   }
+
+@[user_command]
+meta def puddle_def (meta_info : decl_meta_info) (_ : parse $ tk "pdef") : lean.parser unit :=
+do i ← ident,
+   tk ":=",
+   return ().
+
+end puddle_def
+end puddle
+
+pdef try_mix :=
+
